Working implementation for Pawn, En Passant, and Rook moves

board.dfy
@@ -3,7 +3,7 @@ datatype Piece = Pawn | Bishop | Knight | Rook | Queen | King
 datatype Cell = Empty | Piece(color: Color, piece: Piece, moved: bool)
 
 datatype Move = PieceMove(from: (int, int), to: (int, int), capture: bool) 
-                | Castle(color: Color, kingside: bool)
+                | Castle(color: Color, kingside: bool) | EnPassant(from: (int, int), to: (int, int), color: Color) | PawnPromotion(from: (int, int), to: (int, int), color: Color, newPiece: Piece)
 
 class Board {
     // I treat the grid as a row-major 2D array. The rows of the array
@@ -12,17 +12,21 @@ class Board {
     // order. E.g. column 0 is file A and row 0 is rank 1.
     var grid: array2<Cell>
 
+    // Keep track of moves for special cases like en passant
+    var moves: seq<Move>
+
     function class_invariant(): bool
         reads this, grid
     {
         grid.Length0 == 8 &&
-        grid.Length1 == 8
+        grid.Length1 == 8 &&
+        |moves| >= 0
         // TODO: Number of each color's kings is exactly one.
         // Optional: We can make sure each piece count is not above a certain
         // amount.
     }
 
-    // Helper function for initial_board.
+    // Helper function for creating the initial_board.
     static function piece_at(i: int, j: int): Piece
         requires 0 <= i < 8
         requires 0 <= j < 8
@@ -50,13 +54,15 @@ class Board {
 
     constructor()
         ensures class_invariant() && fresh(grid)
+        ensures forall i, j :: 0 <= i < grid.Length0 && 0 <= j < grid.Length1 ==> grid[i, j] == initial_board(i, j)
     {
         grid := new Cell[8, 8](initial_board);
+        moves := [];
     }
 
     // Is the given move in the right range of the board?
     function MoveInRange(move: Move): bool
-        requires move.PieceMove?
+        requires move.PieceMove? || move.EnPassant?
     {
         0 <= move.from.0 < 8 &&
         0 <= move.from.1 < 8 &&
@@ -64,12 +70,14 @@ class Board {
         0 <= move.to.1 < 8
     }
 
+    // This is a precondition for a normal move, to and from must be in bounds,
+    // the source cell must have a piece, and the destination cell must be empty
     function NoCapturePre(move: Move): bool
         requires move.PieceMove? && !move.capture
         reads this, grid
         requires class_invariant()
+        requires MoveInRange(move)
     {
-        && MoveInRange(move)
         && grid[move.from.0, move.from.1] != Empty
         && grid[move.to.0, move.to.1] == Empty
     }
@@ -77,8 +85,10 @@ class Board {
     // Does this move describe a valid capture on the board?
     // TODO: Exceptions for en passant.
     function CapturePre(move: Move): bool
-        requires move.PieceMove? && move.capture
+        requires move.PieceMove? || move.EnPassant?
+        requires move.PieceMove? ==> move.capture
         reads this, grid
+        requires MoveInRange(move)
         requires class_invariant()
     {
         && MoveInRange(move)
@@ -89,6 +99,8 @@ class Board {
     }
 
     // Is the board in the expected state after making the move?
+    // Have NO OTHER cells been modified?
+    // TODO: Conditions for En Passant, Castling
     function PieceMovePost(move: Move, cell: Cell): bool
         requires move.PieceMove?
         reads this, grid
@@ -142,30 +154,240 @@ class Board {
         )
     }
 
+    predicate PiecePre(move: Move, piece: Piece)
+    reads this, this.grid
+    {
+        move.PieceMove? &&
+        class_invariant() &&
+        MoveInRange(move) &&
+        (move.capture == false ==> NoCapturePre(move)) &&
+        (move.capture == true ==> CapturePre(move)) &&
+        
+        grid[move.from.0, move.from.1] != Empty &&
+        grid[move.from.0, move.from.1].piece == Pawn &&
+        grid[move.to.0, move.to.1] == Empty
+    }
+
+    predicate PawnPre(move: Move)
+        reads this, this.grid
+        requires PiecePre(move, Pawn)
+    {
+        var cell := grid[move.from.0, move.from.1];
+        var color := cell.color;
+        var from := move.from;
+        var to := move.to;
+
+        match color
+        case White =>
+            // Forward direction: increase rank (row number)
+            if !move.capture then
+                (to.1 == from.1) &&
+                (
+                    (to.0 == from.0 + 1) || // single step
+                    (from.0 == 1 && to.0 == from.0 + 2 && grid[from.0 + 1, from.1] == Empty) // double step from start
+                )
+            else // Pawn capture case
+                (to.0 == from.0 + 1) && // Moves up a row
+                (to.1 == from.1 + 1 || to.1 == from.1 - 1) && // Moves Diagonal 1
+                (grid[to.0, to.1] != Empty) // There's a piece at the destination
+        case Black =>
+            if !move.capture then
+                (to.1 == from.1) &&
+                (
+                (to.0 == from.0 - 1) ||
+                (from.0 == 6 && to.0 == from.0 - 2 && grid[from.0 - 1, from.1] == Empty))
+            else
+                (to.0 == from.0 - 1) &&
+                (to.1 == from.1 + 1 || to.1 == from.1 - 1) &&
+                grid[to.0, to.1] != Empty
+    }
+
+    predicate RookPre(move: Move)
+        reads this, this.grid
+        requires PiecePre(move, Rook)
+    {
+        var from := move.from;
+        var to := move.to;
+        var fromCell := grid[from.0, from.1];
+        // 1. Establish Direction
+        // 2. Ensure that everything on the way to the destination is free (if not a capture), else last space must have a piece
+        // for each direction
+        if to.0 > from.0 && to.1 == from.1 // UP (from increasing)
+        then 
+            (move.capture &&
+            (forall i :: from.0 < i < to.0 ==> grid[i, to.1] == Empty) &&
+            grid[to.0, to.1] != Empty &&
+            grid[to.0, to.1].color != fromCell.color
+            ) ||
+            (!move.capture &&
+            (forall i :: from.0 < i <= to.0 ==> grid[i, to.1] == Empty))
+        else if to.0 < from.0 && to.1 == from.1 // DOWN
+        then
+            (move.capture &&
+            (forall i :: to.0 < i < from.0 ==> grid[i, to.1] == Empty) &&
+            grid[to.0, to.1] != Empty &&
+            grid[to.0, to.1].color != fromCell.color
+            ) ||
+            (!move.capture &&
+            (forall i :: to.0 <= i < from.0 ==> grid[i, to.1] == Empty))
+        else if to.1 > from.1 && to.0 == from.0 // RIGHT
+        then
+            (move.capture &&
+            (forall i :: from.1 < i < to.1 ==> grid[to.0, i] == Empty) &&
+            grid[to.0, to.1] != Empty &&
+            grid[to.0, to.1].color != fromCell.color
+            ) ||
+            (!move.capture &&
+            (forall i :: from.1 < i <= to.1 ==> grid[to.0, i] == Empty))
+        else if to.1 < from.1 && to.0 == from.0 // LEFT
+        then
+            (move.capture &&
+            (forall i :: to.1 < i < from.1 ==> grid[to.0, i] == Empty) &&
+            grid[to.0, to.1] != Empty &&
+            grid[to.0, to.1].color != fromCell.color
+            ) ||
+            (!move.capture &&
+            (forall i :: to.1 <= i < from.1 ==> grid[to.0, i] == Empty))
+        else false
+    }
+
+    predicate LegalMoveChecker(move: Move)
+    reads this, grid
+    requires class_invariant()
+    requires move.PieceMove? || move.EnPassant? ==> MoveInRange(move)
+    {
+        match move
+        case PieceMove(from, to, capture) =>
+            MoveInRange(move) &&
+            (capture ==>
+                CapturePre(move)
+            ) &&
+            (!capture ==>
+                NoCapturePre(move) &&
+                ((grid[from.0, from.1].piece == Pawn ==>
+                    PawnPre(move)
+                ) ||
+                (grid[from.0, from.1].piece == Rook ==>
+                    RookPre(move)))
+                // TODO: Other Pieces
+            )
+        case Castle(color, kingside) =>
+            CastlePre(move)
+        case EnPassant(from, to, color) =>
+            // true
+            EnPassantPre(move) // Not yet implemented
+        case PawnPromotion(_, _, _, _) =>
+            false // Not yet implemented
+    }
+
+    predicate EnPassantPre(move: Move)
+    reads this, this.grid
+    requires class_invariant()
+    requires move.EnPassant?
+    requires MoveInRange(move)
+    {
+
+        var from := move.from;
+        var to := move.to;
+        var cell := grid[from.0, from.1];
+        var color := move.color;
+
+        cell != Empty &&
+        cell.piece == Pawn &&
+        grid[to.0, to.1] == Empty &&
+
+        if color == White then
+            from.0 == 4 && // White must be on rank 5
+            to.0 == 5 &&
+            (to.1 == from.1 + 1 || to.1 == from.1 - 1) &&
+            // The captured pawn must be a Black pawn
+            var capturedCol := to.1;
+            grid[4, capturedCol] == Piece(Black, Pawn, true) &&
+            |moves| > 0 &&
+            moves[|moves| - 1] == PieceMove((6, capturedCol), (4, capturedCol), false)
+        else
+            from.0 == 3 && // Black must be on rank 4
+            to.0 == 2 &&
+            (to.1 == from.1 + 1 || to.1 == from.1 - 1) &&
+            var capturedCol := to.1;
+            // The captured pawn must be a White pawn
+            grid[3, capturedCol] == Piece(White, Pawn, true) &&
+            |moves| > 0 &&
+            moves[|moves| - 1] == PieceMove((1, capturedCol), (3, capturedCol), false)
+    }
+
+    function EnPassantPost(move: Move, oldGrid: array2<Cell>): bool
+    requires move.EnPassant?
+    reads this, this.grid, oldGrid
+    requires class_invariant()
+    requires MoveInRange(move)
+    requires this.grid.Length0 == oldGrid.Length0 && this.grid.Length1 == oldGrid.Length1
+    {
+        var from := move.from;
+        var to := move.to;
+        var fromCell := grid[from.0, from.1];
+        var toCell := grid[to.0, to.1];
+        var capturedCell := grid[from.0, to.1];
+        // assume this.grid.Length0 == oldGrid.Length0 && this.grid.Length1 == oldGrid.Length1;
+
+        // Check the pawn has moved to the destination
+        toCell != Empty &&
+        toCell.piece == Pawn &&
+        ((move.color == White && toCell.color == White) || ((move.color == Black) && toCell.color == Black)) &&
+        toCell.moved == true &&
+        fromCell == Empty &&
+        // The captured pawn has been removed
+        grid[from.0, to.1] == Empty &&
+        // All other squares have been unchanged
+        forall i, j :: 0 <= i < grid.Length0 && 0 <= j < grid.Length1 && (i, j) != (from.0, from.1) && (i, j) != (to.0, to.1) && (i, j) != (from.0, to.1) ==> this.grid[i, j] == oldGrid[i, j]
+    }
+
     // TODO: Verify counts of pieces. Actually, we need to ensure that all
     // other pieces are unchanged.
     method MakeMove(move: Move)
+        modifies this, grid
         requires class_invariant()
-        modifies grid
-
-        requires move.PieceMove? && !move.capture ==> NoCapturePre(move)
-        requires move.PieceMove? && move.capture ==> CapturePre(move)
-        requires move.Castle? ==> CastlePre(move)
+        requires move.PieceMove? || move.EnPassant? ==> MoveInRange(move)
+        requires LegalMoveChecker(move)
 
         ensures class_invariant()
-        ensures old(grid) == grid // Reference is unchanged.
+        ensures move.PieceMove? ==> PieceMovePost(move, old(grid[move.from.0, move.from.1]))
+        ensures move.Castle? ==> CastlePost(move)
+        ensures move.EnPassant? ==> EnPassantPost(move, old(this.grid))
+        ensures move.EnPassant? ==> 
+            forall i, j :: 0 <= i < grid.Length0 && 0 <= j < grid.Length1 && (i, j) != (move.from.0, move.from.1) && (i, j) != (move.to.0, move.to.1) && (i, j) != (move.from.0, move.to.1) ==> grid[i, j] == old(grid[i, j])
 
-        ensures move.PieceMove? ==>
-            PieceMovePost(move, old(grid[move.from.0, move.from.1]))
-        ensures move.Castle? ==>
-            CastlePost(move)
+        ensures this.moves == old(this.moves) + [move]
+        ensures this.grid == old(this.grid) // Needed for some reason
+
+        // Ensure NOTHING ELSE CHANGED IN THE BOARD
+        ensures move.PieceMove? ==> forall i, j :: 0 <= i < this.grid.Length0 && 0 <= j < this.grid.Length1 && (i, j) != move.from && (i, j) != move.to ==> this.grid[i, j] == old(this.grid[i, j])
+
+        // TODO: Ensure nothing else changed in the board for Castle, then En Passant
+
+        // Ensure the move was added, and that the rest of the sequence is the same
+        ensures this.moves == old(this.moves) + [move]
+        ensures |this.moves| == old(|this.moves|) + 1
+        ensures this.moves[|this.moves| - 1] == move
+        ensures |this.moves| > 0 ==> forall i:int :: 0 <= i < |this.moves| - 1 ==> this.moves[i] == old(this.moves[i])
     {
         if move.PieceMove? {
             var cell := grid[move.from.0, move.from.1];
-            grid[move.to.0, move.to.1] := Piece(
-                cell.color, cell.piece, true
-            );
-            grid[move.from.0, move.from.1] := Empty;
+
+            match cell.piece
+            case Pawn =>
+                // Pretty much the lemmas / predicates go here
+                var cell := grid[move.from.0, move.from.1];
+                grid[move.to.0, move.to.1] := Piece(
+                    cell.color, cell.piece, true
+                );
+                grid[move.from.0, move.from.1] := Empty;
+            case _ =>
+                var cell := grid[move.from.0, move.from.1];
+                grid[move.to.0, move.to.1] := Piece(
+                    cell.color, cell.piece, true
+                );
+                grid[move.from.0, move.from.1] := Empty;
         } else if move.Castle? {
             var rank := if move.color == White then 0 else 7;
             var rookfile := if move.kingside then 7 else 0;
@@ -179,7 +401,31 @@ class Board {
                 grid[rank, 3] := Piece(move.color, Rook, true);
             }
             grid[rank, 4] := Empty;
+        } else if move.EnPassant? {
+            var cell := grid[move.from.0, move.from.1];
+            var from := move.from;
+            var to := move.to;
+
+            match cell.color
+            case White =>
+                // 1. Move White Pawn
+                grid[to.0, to.1] := Piece(move.color, Pawn, true);
+                grid[from.0, from.1] := Empty;
+
+                // 2. Capture Black Pawn (Just set it to empty for now TODO)
+                grid[from.0, to.1] := Empty;
+
+            case Black =>
+                // 1. Move Black Pawn
+                grid[to.0, to.1] := Piece(move.color, Pawn, true);
+                grid[from.0, from.1] := Empty;
+
+                // 2. Capture White Pawn
+                grid[from.0, to.1] := Empty;
         }
+
+        // Add the move to the moves list
+        this.moves := this.moves + [move];
     }
 
     method ParseMove(s: string) returns (move: Move)
@@ -200,19 +446,114 @@ method TestBoard() {
     board.grid[7, 7] := Piece(Black, Rook, false);
     board.grid[0, 5] := Empty;
     board.grid[0, 6] := Empty;
-    //board.grid[7, 7] := Empty;
-    //board.MakeMove(PieceMove((0, 0), (7, 7), false));
-    //assert board.grid[0, 0] == Empty;
+    // board.grid[7, 7] := Empty;
+    // board.MakeMove(PieceMove((0, 0), (7, 7), false));
+    // assert board.grid[0, 0] == Empty;
     //assert board.grid[7, 7] != Empty;
     //assert board.grid[7, 7].color == White;
     //assert board.grid[7, 7].piece == Rook;
     //assert board.grid[7, 7].moved == true;
 
-    //assert board.grid[7, 7] == Piece(White, Rook, true);
+    // //assert board.grid[7, 7] == Piece(White, Rook, true);
 
-    board.grid[0, 4] := Piece(White, King, false);
-    board.grid[7, 4] := Piece(Black, King, false);
+    // board.grid[0, 4] := Piece(White, King, false);
+    // board.grid[7, 4] := Piece(Black, King, false);
 
-    board.MakeMove(Castle(White, true));
+    // board.MakeMove(Castle(White, true));
     //board.MakeMove(Castle(White, false));
+
+    // Test Pawn Normal Moves
+    var pawns := new Board();
+    var move := PieceMove((1,0), (2,0), false);
+    // assert forall i, j :: 0 <= i < pawns.grid.Length0 && 0 <= j < pawns.grid.Length1 ==> pawns.grid[i, j] == pawns.initial_board(i, j);
+    // assert pawns.grid[1, 0].Piece?;
+    // assert pawns.grid[1, 0].piece == Pawn;
+    // assert pawns.grid[2, 0].Empty?;
+    pawns.MakeMove(move);
+    assert pawns.grid[2, 0].piece == Pawn;
+    assert pawns.grid[1, 0].Empty?;
+    move := PieceMove((2,0), (3,0), false);
+    pawns.MakeMove(move);
+    assert pawns.grid[3, 0].piece == Pawn;
+    // move := PieceMove((3,0), (5,0), false);
+    // pawns.MakeMove(move); // This fails (as it should since it's an invalid move)
+
+    move := PieceMove((1,1), (3,1), false);
+    pawns.MakeMove(move);
+    assert pawns.grid[1, 1].Empty?;
+    assert pawns.grid[3,1].piece == Pawn;
+    assert pawns.moves[|pawns.moves| - 1] == move; // we really only care about the last move
+
+    move := PieceMove((6,1), (4,1), false);
+    pawns.MakeMove(move);
+    assert pawns.grid[6,1].Empty?;
+    assert pawns.grid[4, 1].piece == Pawn;
+
+    //// Test Pawn Capture Moves
+
+    var pawnCapture := new Board();
+    pawnCapture.grid[2,1] := Piece(Black, Pawn, false);
+    move := PieceMove((1,0), (2,1), true);
+    pawnCapture.MakeMove(move);
+    assert pawnCapture.grid[2,1].color == White;
+    assert pawnCapture.grid[1, 0].Empty?;
+
+    pawnCapture.grid[6,3] := Piece(White, Queen, false);
+    move := PieceMove((7,2), (6,3), true);
+    pawnCapture.MakeMove(move);
+    assert pawnCapture.grid[6,3].color == Black;
+    assert pawnCapture.grid[7,2].Empty?;
+
+    // En Passant Tester
+    var pawnEnPassant := new Board();
+    move := PieceMove((1,0), (3,0), false);
+    // Move
+    pawnEnPassant.MakeMove(move);
+    move := PieceMove((3,0), (4,0), false);
+    pawnEnPassant.MakeMove(move);
+    // Black pawn moves forward 2, opening up En Passant for white pawn at 4,0
+    move := PieceMove((6,1), (4,1), false);
+    pawnEnPassant.MakeMove(move);
+    assert pawnEnPassant.grid[4,1].color == Black;
+    assert pawnEnPassant.grid[4,0].color == White;
+
+    move := EnPassant((4,0), (5,1), White);
+    pawnEnPassant.MakeMove(move);
+    assert pawnEnPassant.grid[4,1].Empty?;
+    assert pawnEnPassant.grid[5,1].color == White;
+    assert pawnEnPassant.grid[6, 6].color == Black; // Making sure some random piece is still in the right spot
+    assert pawnEnPassant.grid[7,0].piece == Rook;
+
+    // Move a random piece
+    pawnEnPassant.MakeMove(PieceMove((7,1), (6,1), false));
+    assert pawnEnPassant.grid[6,1].color == Black;
+
+    // Test Black En Passant
+    pawnEnPassant.MakeMove(PieceMove((6, 5), (4, 5), false)); // Black Pawn forward 2
+    pawnEnPassant.MakeMove(PieceMove((4, 5), (3, 5), false)); // Black Pawn forward 1
+    pawnEnPassant.MakeMove(PieceMove((1, 6), (3, 6), false)); // White Pawn forward 2 (Black is now setup for en passant)
+    pawnEnPassant.MakeMove(EnPassant((3, 5), (2, 6), Black)); // Black En Passant
+    assert pawnEnPassant.grid[2,6].color == Black;
+    assert pawnEnPassant.grid[2,6].piece == Pawn;
+    assert pawnEnPassant.grid[3,6].Empty?;
+
+    // Move a random piece (this captures)
+    pawnEnPassant.MakeMove(PieceMove((6,1), (5,1), true));
+    assert pawnEnPassant.grid[5,1].color == Black;
+
+    // Testing Rook
+    var rookTest := new Board();
+    // Move pawns out of the way
+    rookTest.MakeMove(PieceMove((6,0), (4,0), false)); // Move left black pawn down
+    rookTest.MakeMove(PieceMove((1,0), (3,0), false)); // Move left white pawn up
+
+    rookTest.MakeMove(PieceMove((0,0), (2,0), false)); // Move left white rook up
+    rookTest.MakeMove(PieceMove((7,0), (5,0), false)); // Move left black rook down
+    assert rookTest.grid[2,0].color == White && rookTest.grid[2,0].piece == Rook;
+    assert rookTest.grid[5,0].color == Black && rookTest.grid[5,0].piece == Rook;
+
+    // Testing Rook Capture
+    rookTest.MakeMove(PieceMove((5,0), (5,5), false)); // Move left black rook right
+    rookTest.MakeMove(PieceMove((5,5), (1,5), true)); // Move left black rook down and capture a pawn
+    assert rookTest.grid[1,5].color == Black && rookTest.grid[1,5].piece == Rook;
 }
